work on partial liveness maps

systems/FailureRecorderStaticLabeled.v
@@ -61,6 +61,10 @@ Inductive Label : Type :=
 | Tau : Label
 | RecvFail : name -> name -> Label.
 
+Definition Label_eq_dec : forall x y : Label, {x = y} + {x <> y}.
+decide equality; exact: name_eq_dec.
+Defined.
+
 Definition Handler (S : Type) := GenHandler (name * Msg) S Output Label.
 
 Definition NetHandler (me src: name) (msg : Msg) : Handler Data :=
@@ -90,6 +94,7 @@ Instance FailureRecorder_LabeledMultiParams : LabeledMultiParams FailureRecorder
     lb_all_names_nodes := all_names_nodes ;
     lb_no_dup_nodes := no_dup_nodes ;
     label := Label ;
+    label_eq_dec := Label_eq_dec ;
     label_silent := Tau ;
     lb_init_handlers := InitData ;
     lb_net_handlers := (fun dst src msg s => runGenHandler s (NetHandler dst src msg)) ;
