core/PartialMapLivenessSimulations.v
@@ -1,0 +1,251 @@
+Require Import List.
+Import ListNotations.
+
+Require Import Arith.
+Require Import ZArith.
+Require Import Omega.
+
+Require Import StructTact.StructTactics.
+Require Import HandlerMonad.
+Require Import Net.
+Require Import LabeledNet.
+Require Import StructTact.Util.
+Require Import FunctionalExtensionality.
+
+Require Import TotalMapSimulations.
+Require Import PartialMapSimulations.
+Require Import TotalMapLivenessSimulations.
+Require Import infseq.
+
+Local Arguments update {_} {_} {_} _ _ _ _ : simpl never.
+
+Require Import mathcomp.ssreflect.ssreflect.
+Require Import mathcomp.ssreflect.ssrbool.
+
+Set Implicit Arguments.
+
+Class LabeledMultiParamsPartialMapCongruency
+  (B0 : BaseParams) (B1 : BaseParams)
+  (P0 : LabeledMultiParams B0) (P1 : LabeledMultiParams B1)
+  (B : BaseParamsPartialMap B0 B1) 
+  (N : MultiParamsNameTotalMap (@unlabeled_multi_params _ P0) (@unlabeled_multi_params _ P1))
+  (P : MultiParamsMsgPartialMap (@unlabeled_multi_params _ P0) (@unlabeled_multi_params _ P1))
+  (L : LabeledMultiParamsLabelTotalMap P0 P1) :=
+  {
+    pt_lb_label_silent_fst_snd : tot_map_label label_silent = label_silent ;
+    pt_lb_net_handlers_some : forall me src m st m' out st' ps lb,
+      pt_map_msg m = Some m' ->
+      lb_net_handlers (tot_map_name me) (tot_map_name src) m' (pt_map_data st) = (lb, out, st', ps) ->
+      lb <> label_silent /\ tot_mapped_lb_net_handlers_label me src m st = lb ;
+    pt_lb_net_handlers_none : forall me src m st,
+      pt_map_msg m = None ->
+      tot_mapped_lb_net_handlers_label me src m st = label_silent ;
+    pt_lb_input_handlers_some : forall me inp st inp' out st' ps lb,
+      pt_map_input inp = Some inp' ->
+      lb_input_handlers (tot_map_name me) inp' (pt_map_data st) = (lb, out, st', ps) ->
+      lb <> label_silent /\ tot_mapped_lb_input_handlers_label me inp st = lb ;
+    pt_lb_input_handlers_none : forall me inp st,
+      pt_map_input inp = None ->
+      tot_mapped_lb_input_handlers_label me inp st = label_silent
+  }.
+
+Section PartialMapLivenessSimulations.
+
+Context {base_fst : BaseParams}.
+Context {base_snd : BaseParams}.
+Context {labeled_multi_fst : LabeledMultiParams base_fst}.
+Context {labeled_multi_snd : LabeledMultiParams base_snd}.
+Context {base_map : BaseParamsPartialMap base_fst base_snd}.
+Context {name_map : MultiParamsNameTotalMap (@unlabeled_multi_params _ labeled_multi_fst) (@unlabeled_multi_params _ labeled_multi_snd)}.
+Context {msg_map : MultiParamsMsgPartialMap (@unlabeled_multi_params _ labeled_multi_fst) (@unlabeled_multi_params _ labeled_multi_snd)}.
+Context {label_map : LabeledMultiParamsLabelTotalMap labeled_multi_fst labeled_multi_snd}.
+Context {name_map_bijective : MultiParamsNameTotalMapBijective name_map}.
+Context {multi_map_congr : MultiParamsPartialMapCongruency base_map name_map msg_map}.
+Context {multi_map_lb_congr : LabeledMultiParamsPartialMapCongruency base_map name_map msg_map label_map}.
+
+Theorem lb_step_f_pt_mapped_simulation_1_non_silent :
+  forall net net' failed failed' lb tr,
+    tot_map_label lb <> label_silent ->
+    @lb_step_f _ labeled_multi_fst (failed, net) lb (failed', net') tr ->
+    @lb_step_f _ labeled_multi_snd (map tot_map_name failed, pt_map_net net) (tot_map_label lb) (map tot_map_name failed', pt_map_net net') (pt_map_trace tr).
+Proof.
+move => net net' failed failed' lb tr H_neq H_step.
+have H_neq': lb <> label_silent.
+  rewrite -pt_lb_label_silent_fst_snd in H_neq.
+  move => H_eq.
+  by rewrite H_eq in H_neq.
+invcs H_step => //=.
+- case H_m: (pt_map_packet p) => [p'|]; last first.
+    destruct p.
+    simpl in *.
+    break_match => //.
+    have H_q := @pt_lb_net_handlers_none _ _ _ _ _ _ _ _ multi_map_lb_congr pDst pSrc _ (nwState net pDst) Heqo.
+    rewrite /tot_mapped_lb_net_handlers_label in H_q.
+    repeat break_let.
+    by tuple_inversion.
+  have H_eq_n: tot_map_name (pDst p) = pDst p'.
+    destruct p.
+    simpl in *.
+    break_match => //.
+    by find_injection.
+  rewrite H_eq_n.
+  apply (@LSF_deliver _ _ _ _ _ _ (pt_map_packets xs) (pt_map_packets ys) (pt_map_outputs out) (pt_map_data d) (@pt_map_name_msgs _ _ _ _ _ msg_map l)).
+  * rewrite /pt_map_net /=.
+    find_rewrite.
+    by rewrite pt_map_packets_app_distr /= H_m.
+  * rewrite -H_eq_n.
+    exact: not_in_failed_not_in.
+  * rewrite /pt_map_net /= -{2}H_eq_n tot_map_name_inv_inverse.
+    destruct p, p'.
+    simpl in *.
+    break_match => //.
+    find_injection.
+    clean.
+    have H_q := @pt_net_handlers_some _ _ _ _ _ _ _ multi_map_congr pDst pSrc pBody (nwState net pDst) _ Heqo.
+    rewrite /pt_mapped_net_handlers /net_handlers /= /unlabeled_net_handlers in H_q.
+    repeat break_let.
+    repeat tuple_inversion.
+    have H_q' := @pt_lb_net_handlers_some _ _ _ _ _ _ _ _ multi_map_lb_congr _ _ _ _ _ _ _ _ _ Heqo Heqp1.
+    rewrite /tot_mapped_lb_net_handlers_label in H_q'.
+    repeat break_let.
+    break_and.
+    by repeat tuple_inversion.
+  * rewrite /pt_map_net /= 2!pt_map_packets_app_distr.
+    by rewrite (pt_map_packet_map_eq_some _ _ H_m) (pt_map_update_eq_some _ _ _ H_m).
+- case H_i: pt_map_input => [inp'|]; last first.
+    have H_q := @pt_lb_input_handlers_none _ _ _ _ _ _ _ _ multi_map_lb_congr h _ (nwState net h) H_i.
+    rewrite /tot_mapped_lb_input_handlers_label /= in H_q.
+    repeat break_let.
+    by tuple_inversion.
+  apply (@LSF_input _ _ _ _ _ _ _ _ (pt_map_data d) (@pt_map_name_msgs _ _ _ _ _ msg_map l)).
+  * exact: not_in_failed_not_in.
+  * have H_q := @pt_input_handlers_some _ _ _ _ _ _ _ multi_map_congr h _ (nwState net h) _ H_i.
+    rewrite /pt_mapped_input_handlers /input_handlers /= /unlabeled_input_handlers in H_q.
+    repeat break_let.
+    repeat tuple_inversion.
+    have H_q' := @pt_lb_input_handlers_some _ _ _ _ _ _ _ _ multi_map_lb_congr _ _ _ _ _ _ _ _ H_i Heqp1.
+    break_and.
+    unfold tot_mapped_lb_input_handlers_label in *.
+    repeat break_let.
+    repeat tuple_inversion.
+    by rewrite /pt_map_net /= tot_map_name_inv_inverse.
+  * rewrite /pt_map_net /=.
+    rewrite pt_map_packets_app_distr pt_map_packet_map_eq.
+    by rewrite -pt_map_update_eq.
+Qed.
+
+Theorem lb_step_f_pt_mapped_simulation_1_silent :
+  forall net net' failed failed' lb tr,
+    tot_map_label lb = label_silent ->
+    @lb_step_f _ labeled_multi_fst (failed, net) lb (failed', net') tr ->
+    @lb_step_f _ labeled_multi_snd (map tot_map_name failed, pt_map_net net) label_silent (map tot_map_name failed', pt_map_net net') [].
+Proof.
+move => net net' failed failed' lb tr H_eq H_step.
+invcs H_step => //=.
+- case H_m: (pt_map_packet p) => [p'|].
+    destruct p, p'.
+    simpl in *.
+    break_match => //.
+    find_injection.
+    have H_q := @pt_net_handlers_some _ _ _ _ _ _ _ multi_map_congr pDst pSrc pBody (nwState net pDst) _ Heqo.
+    rewrite /pt_mapped_net_handlers /net_handlers /= /unlabeled_net_handlers in H_q.
+    repeat break_let.
+    repeat tuple_inversion.
+    have H_q' := @pt_lb_net_handlers_some _ _ _ _ _ _ _ _ multi_map_lb_congr _ _ _ _ _ _ _ _ _ Heqo Heqp1.
+    break_and.
+    unfold tot_mapped_lb_net_handlers_label in *.
+    repeat break_let.
+    by repeat tuple_inversion.
+  destruct p.
+  simpl in *.
+  break_match => //.
+  have H_q := @pt_net_handlers_none _ _ _ _ _ _ _ multi_map_congr pDst pSrc pBody (nwState net pDst) out d l Heqo.
+  rewrite /net_handlers /= /unlabeled_net_handlers in H_q.
+  repeat break_let.
+  repeat tuple_inversion.
+  concludes.
+  break_and.
+  have H_q' := @pt_lb_net_handlers_none _ _ _ _ _ _ _ _ multi_map_lb_congr pDst pSrc _ (nwState net pDst) Heqo.
+  rewrite /tot_mapped_lb_net_handlers_label in H_q'.
+  repeat break_let.
+  repeat tuple_inversion.
+  rewrite /pt_map_net /=.
+  rewrite pt_map_packets_app_distr.
+  rewrite pt_map_name_msgs_empty_eq //=.
+  rewrite H3.
+  rewrite pt_map_packets_app_distr /=.
+  repeat break_match => //.
+  rewrite -pt_map_packets_app_distr.
+  set s1 := fun _ => _.
+  set s2 := fun _ => _.
+  have H_eq_s: s1 = s2.
+    rewrite /s1 /s2.
+    apply functional_extensionality => n.
+    rewrite /update.
+    by break_if; first by rewrite H e.
+  rewrite -H_eq_s /s1 {s1 s2 H_eq_s}.
+  exact: LSF_stutter.
+- case H_i: (pt_map_input inp) => [inp'|].
+    have H_q := @pt_input_handlers_some _ _ _ _ _ _ _ multi_map_congr h _ (nwState net h) _ H_i.
+    rewrite /pt_mapped_input_handlers /input_handlers /= /unlabeled_input_handlers in H_q.
+    repeat break_let.
+    repeat tuple_inversion.
+    have H_q' := @pt_lb_input_handlers_some _ _ _ _ _ _ _ _ multi_map_lb_congr _ _ _ _ _ _ _ _ H_i Heqp1.
+    break_and.
+    unfold tot_mapped_lb_input_handlers_label in *.
+    repeat break_let.
+    by tuple_inversion.
+  have H_q := @pt_input_handlers_none _ _ _ _ _ _ _ multi_map_congr h _ (nwState net h) out d l H_i.
+  rewrite /input_handlers /= /unlabeled_input_handlers in H_q.
+  repeat break_let.
+  repeat tuple_inversion.
+  concludes.
+  break_and.
+  have H_q' := @pt_lb_input_handlers_none _ _ _ _ _ _ _ _ multi_map_lb_congr h _ (nwState net h) H_i.
+  rewrite /tot_mapped_lb_input_handlers_label in H_q'.
+  repeat break_let.
+  repeat tuple_inversion.
+  rewrite /pt_map_net /=.
+  rewrite pt_map_packets_app_distr.
+  rewrite pt_map_name_msgs_empty_eq //=.
+  set s1 := fun _ => _.
+  set s2 := fun _ => _.
+  have H_eq_s: s1 = s2.
+    rewrite /s1 /s2.
+    apply functional_extensionality => n.
+    rewrite /update.
+    by break_if; first by rewrite H e.
+  rewrite -H_eq_s /s1 {s1 s2 H_eq_s}.
+  exact: LSF_stutter.
+- exact: LSF_stutter.
+Qed.
+
+Definition pt_map_event e : event _ _ _ := 
+((map tot_map_name (fst (a_of_event e)), pt_map_net (snd (a_of_event e))), tot_map_label (l_of_event e), pt_map_trace (tr_of_event e)).
+
+(*
+Definition select lb 
+ (tr : list (@name _ (@unlabeled_multi_params _ labeled_multi_fst) * (@input base_fst + list (@output base_fst)))) 
+ (s : infseq (event (list (@name _ (@unlabeled_multi_params _ labeled_multi_fst)) * 
+                     (@network _ (@unlabeled_multi_params _ labeled_multi_fst))) (@label _ labeled_multi_fst) _)) :=
+if label_eq_dec (tot_map_label lb) label_silent then tr else tr_of_event (hd s).
+
+CoFixpoint pt_map_infseq s tr :=
+match s with
+| Cons e s' => Cons (pt_map_event ((a_of_event e), (l_of_event e), tr)) (pt_map_infseq s' (select (l_of_event e) tr s'))
+end.
+
+Lemma pt_map_infseq_unfold : forall s tr,
+    Cons (pt_map_event (a_of_event (hd s), l_of_event (hd s), tr)) (pt_map_infseq (tl s) (select (l_of_event (hd s)) tr (tl s))) = 
+    pt_map_infseq s tr.
+Proof.
+Admitted.
+
+Lemma lb_step_execution_lb_step_f_pt_map_infeq : forall s,
+  lb_step_execution lb_step_f s  ->
+  lb_step_execution lb_step_f (pt_map_infseq s (tr_of_event (hd s))).
+Proof.
+Admitted.
+*)
+
+End PartialMapLivenessSimulations.
